---
tags:
  - MAE376
due: 2026-02-13
submitted: T
src:
---
by Joseph Ramirez

1
$$L\{e^{4t}+5\}=L\{e^{4t}\}+L\{5\}$$
$$=\frac{1}{s-4}+\frac{5}{s}$$

2
$$L\{\cos{2t}+7\sin{2t}\}=L\{\cos{2t}\}+L\{7\sin 2t\}$$
$$=\frac{s}{s^2+4}+\frac{14}{s^2+4}$$

3
$$L\{e^{-2t}\cos{3t}+5e^{-2t}\sin{3t}\}=L\{e^{-2t}\cos{3t}\}+L\{5e^{-2t}\sin{3t}\}$$
$$=\frac{s+2}{(s+2)^2+9}+\frac{5s+10}{(s+2)^2+9}$$

4
$$L\{10+5t+t^2-4t^3\}$$
$$=\frac{10}{s}+\frac{5}{s^2}+\frac{2}{s^3}-\frac{24}{s^4}$$

5
$$L\{(t^2+4t+2)e^{3t}\}$$
$$L\{e^{at}f(t)\}=F(s-a)$$
$$F(s)=\frac{2}{s^3}+\frac{4}{s^2}+\frac{2}{s}$$
$$L\{e^{3t}(t^2+4t+2)\}=\frac{2}{(s-3)^3}+\frac{4}{(s-3)^2}+\frac{2}{s-3}$$

`<div style="page-break-after: always;"></div>

6
$$L\{6e^{5t}\cos{2t}-e^{7t}\}$$
$$=6L\{e^{5t}\cos{2t}\}-L\{e^{7t}\}$$
$$=\frac{6s-30}{(s-5)^2+4}-\frac{1}{s-7}$$
