---
tags:
  - MAE376
due: 2026-03-03
submitted: F
src: https://csulb.instructure.com/courses/117006/assignments/1712602
---
by Joseph Ramirez

1-1
$$F(s)=\frac{e^{-2s}}{s}+\frac{6e^{-3s}}{s}$$
$$f(t)=u_{2}(t)+6u_{3}(t)$$

1-2
$$e^{-3s}\left( \frac{1}{s^2}+\frac{5}{s^3} \right)$$


1-3
$$6+\frac{e^{-s}}{s^2+4}$$

1-4
$$\frac{e^{-5s}(s+1)}{(s+1)^2+16}$$

1-5
$$F(s)=\frac{4e^{-2s}}{s-3}+\frac{e^{-5s}}{s+9}$$

1-6
$$\frac{e^{-10s}}{(s-3)^2}$$

1-7
$$\frac{e^{-7s}}{s}+\frac{e^{-11s}}{(s-2)^3}$$

1-8
$$F(s)=\frac{1}{(s+1)(s^2-1)}$$

1-9
$$F(s)=\frac{2s+3}{s^2+4s+13}$$

1-10
$$F(s)=\frac{e^{-3s}}{s-2}$$

1-11
$$F(s)=\frac{1+e^{-2s}}{s^2+6}$$


2-1
$$f(t)=3u_{6}(t)$$

2-2
$$g(t)=3+7u_{5}(t)-10u_{8}(t)$$

2-3
$$h(t)=6u_{3}(t)\sin(t-3)$$

2-4
$$j(t)=4+5u_{2}(t-2)e^{t-2}$$

2-5
$$u(t)=u_{7}(t)(t-7)^3$$

2-6
$$v(t)=5+u_{1}(t)(t-5)$$

2-7
$$w(t)=2+u_{4}(t)(t^2-2)$$

3. solve the following IVP problem using Laplace transform
3-1
$$y''-1y'+9y=5t^2;\quad y(0)=2;\quad y'(0)=-1$$

3-2
$$y''(t)+4y'(t)=\cos(t)+4t+12;\quad y(0)=0;\quad y'(0)=7$$




