---
tags:
  - MAE376
due: 2026-02-08
submitted: T
src:
---
![[Pasted image 20260208104332.png]]
1a 
$$-\frac{2j}{3-4j}\cdot \frac{3+4j}{3+4j}=\frac{}{}\frac{-6j+8}{9+16}=\frac{8}{25}-\frac{6}{25}j$$
1b 
$$\frac{2j}{3+4j}\cdot \frac{3-4j}{3-4j}=\frac{6j+8}{9+16}=\frac{8}{25}+\frac{6}{25}j$$
$$|\frac{8}{25}-\frac{6}{25}j|=\frac{8}{25}+\frac{6}{25}j$$

2a $$\frac{1-j}{2-\frac{1}{2}j}\cdot \frac{2+\frac{j}{2}}{2+\frac{j}{2}}=\frac{2+\frac{j}{2}-2j+\frac{1}{2}}{4+\frac{1}{4}}=\left( \frac{5}{2}-\frac{3}{2}j \right)\left( \frac{4}{17} \right)=\frac{10}{17}-\frac{6}{17}j$$
2b
$$\frac{|1-j|}{|2-\frac{1}{2}j|}=\frac{1+j}{2+\frac{j}{2}};\quad \frac{1+j}{2+\frac{j}{2}}\cdot \frac{2-\frac{j}{2}}{2-\frac{j}{2}}=\frac{2-\frac{j}{2}+2j+\frac{1}{2}}{4+\frac{1}{4}}=\left( \frac{5}{2}+\frac{3}{2}j \right)\left( \frac{4}{17} \right)=\frac{10}{17}+\frac{6}{17}j$$
$$|\frac{10}{17}-\frac{6}{17}j|=\frac{10}{17}+\frac{6}{17}j$$

`<div style="page-break-after: always;"></div>
![[Pasted image 20260208105037.png]]

5
$$r=\sqrt{ 3+4 }=\sqrt{ 7 }$$
$$\theta=360-\tan^{-1}(\frac{2}{\sqrt{ 3 }})=310.89^{\circ}\to 5.43rad$$
$$z=\sqrt{ 7 }e^{5.43j}$$

6
$$r=\sqrt{ \frac{4}{9}+1 }=\frac{\sqrt{ 13 }}{3}$$
$$\theta=\pi-\tan^{-1}{\frac{1}{\frac{2}{3}}}=2.16rad$$
$$z=\frac{\sqrt{ 13 }}{3}e^{2.16j}$$

8
$$r=\frac{1}{2}$$
$$\theta=\frac{3\pi}{2}$$
$$z=\frac{1}{2}e^{3\pi j/2}$$

 9
$$\frac{1+j}{-1+2j}\to \frac{1+j}{-1+2j}\cdot \frac{-1-2j}{-1-2j}=\frac{-1-2j-j+2}{1+4}=\frac{1}{5}-\frac{3}{5}j$$
$$r=\sqrt{ \frac{1}{25}+\frac{9}{25} }=\frac{\sqrt{ 10 }}{5}$$
$$\theta=2\pi-\tan^{-1}{\frac{\frac{3}{5}}{\frac{1}{5}}}=5.03rad$$
$$z=\frac{\sqrt{ 10 }}{5}e^{5.03j}$$

`<div style="page-break-after: always;"></div>
![[Pasted image 20260208105203.png]]

12
$$r_{1}=\sqrt{ 1+\frac{1}{9} }=\frac{\sqrt{ 10 }}{3};\quad \theta_{1}=2\pi-\tan^{-1}{\frac{1}{3}}=5.96rad$$
$$r_{2}=\sqrt{ \frac{1}{9}+1 }=\frac{\sqrt{ 10 }}{3};\quad \theta_{2}=\tan^{-1}{3}=1.25rad$$
$$\frac{z_{1}}{z_{2}}=\frac{\frac{\sqrt{ 10 }}{3}e^{5.96j}}{\frac{\sqrt{ 10 }}{3}e^{1.25j}}=e^{j(5.96-1.25)}=e^{4.71j}$$
$$r=1;\quad x^2+y^2=1;\quad 4.71rad=270^\circ$$
$$z=-j$$

13
$$\frac{4+j}{(4+3j)^3}$$
$$r_{1}=\sqrt{ 17 };\quad \theta_{1}=\tan^{-1}{\frac{1}{5}}=.197rad$$
$$r_{2}=\sqrt{ 16+9 }=5;\quad \theta_{2}=\tan^{-1}{\frac{3}{4}}=.644rad$$
$$\frac{\sqrt{ 17 }e^{.197j}}{(5e^{.644j})^3}=\frac{\sqrt{ 17 }}{125}e^{j(.197-3*.644)}=.033e^{4.55j}$$
$$x^2+y^2=.033^2$$
$$\tan{4.55rad}=\frac{y}{x}\to y=6.11x$$
$$x^2+(6.11x)^2=.0011$$
$$|x|=\sqrt{ \frac{.0011}{1+6.11^2} }=.00533$$
$$|y|=6.11\cdot .00533=.033$$
$$z=-.00533-.033j$$

15
$$\left( \frac{j}{1+4j} \right)^3$$
$$r_{1}=1;\quad \theta_{1}=1.57rad$$
$$r_{2}=\sqrt{ 17 };\quad \theta_{2}=\tan^{-1}{4}=1.33rad$$
$$(\frac{e^{1.57j}}{\sqrt{ 17 }e^{1.33j}})^3=(.24e^{.24j})^3=.014e^{.73j}$$
$$\sqrt{ x^2+y^2 }=.014$$
$$\tan{.73rad}=\frac{y}{x}\to y=.903x$$
$$x^2+(.903x)^2=.014^2\to x=\sqrt{ \frac{.014^2}{1+.903^2} }=.011$$
$$y=.903\cdot .011=.0096$$
$$z=.011+.0096j$$

`<div style="page-break-after: always;"></div>
![[Pasted image 20260208104425.png]]

16
$$r=\sqrt{ 5 };\quad \theta=\pi-\tan^{-1}{2}=2.03rad$$
$$z=(\sqrt{ 5 }e^{2.03j})^{1/3}=1.31e^{(2k\pi+.68)j}$$

17
$$r=1;\quad \theta=\pi$$
$$-e^{(2k\pi+\pi) j}$$

18
$$(\sqrt{ 3 }-j)^{1/4}$$
$$r=2;\quad \theta=2\pi-\tan^{-1}{\frac{1}{\sqrt{ 3 }}}=\frac{11\pi}{6}$$
$$(2e^{11j\pi/6})^{1/4}=1.19e^{(2k\pi+1.44)j}$$

19
$$\sqrt{ 1+j\sqrt{ 2 } }$$
$$r=\sqrt{ 3 };\quad \theta=\tan^{-1}{\sqrt{ 2 }}=.96rad$$
$$\sqrt{ \sqrt{ 3 }e^{.96j} }=1.32e^{(2k\pi+.48)j}$$


20
$$\left( -\frac{2}{3}+j \right)^{2/3}$$
$$r=\sqrt{ \frac{4}{9}+1 }=1.2;\quad \theta=\pi-\tan^{-1}{\frac{3}{2}}=2.16rad$$
$$(1.2e^{2.16j})^{2/3}=1.13e^{(2k\pi+1.44)j}$$

21
Find all possible roots of $jz^3-(1+j)=0$
$$z^3=\frac{1+j}{j}$$
$$\frac{1+j}{j}\cdot \frac{-j}{-j}=\frac{-j+1}{1}=1-j$$
$$r=\sqrt{ 2 };\quad \theta=2\pi-\tan^{-1}{1}=5.5rad$$
$$z=^{3}\sqrt{ \sqrt{ 2 }e^{5.5j} }=1.12e^{(2k\pi+1.83)j}$$



